Add ATView.v and update ALocal.v

src/attachable/ALocal.v
@@ -19,274 +19,37 @@ Require Import View.
 Require Import Cell.
 Require Import Memory.
 Require Import TView.
+Require Import Local.
+
+Require Import AMemory.
+Require Import ATView.
 
 Set Implicit Arguments.
 
 
-Module ThreadEvent.
-  Inductive t :=
-  | promise (loc:Loc.t) (from to:Time.t) (msg:Message.t) (kind:Memory.op_kind)
-  | silent
-  | read (loc:Loc.t) (ts:Time.t) (val:Const.t) (released:option View.t) (ord:Ordering.t)
-  | write (loc:Loc.t) (from to:Time.t) (val:Const.t) (released:option View.t) (ord:Ordering.t)
-  | update (loc:Loc.t) (tsr tsw:Time.t) (valr valw:Const.t) (releasedr releasedw:option View.t) (ordr ordw:Ordering.t)
-  | fence (ordr ordw:Ordering.t)
-  | syscall (e:Event.t)
-  | failure
-  .
-  Hint Constructors t.
-
-  Inductive kind :=
-  | kind_promise
-  | kind_syscall
-  | kind_others
-  .
-  Hint Constructors kind.
-
-  Definition kinds_all := fun k: kind => True.
-  Hint Unfold kinds_all.
-  Definition kinds_promise := fun k: kind => k = kind_promise.
-  Hint Unfold kinds_promise.
-  Definition kinds_program := fun k: kind => k <> kind_promise.
-  Hint Unfold kinds_program.
-  Definition kinds_tau := fun k: kind => k <> kind_syscall.
-  Hint Unfold kinds_tau.
-
-  Definition get_kind (e:t): kind :=
-    match e with
-    | promise _ _ _ _ _ => kind_promise
-    | syscall _ => kind_syscall
-    | _ => kind_others
-    end.
-
-  Definition get_event (e:t): option Event.t :=
-    match e with
-    | syscall e => Some e
-    | _ => None
-    end.
-
-  Definition get_program_event (e:t): ProgramEvent.t :=
-    match e with
-    | promise _ _ _ _ _  => ProgramEvent.silent
-    | silent => ProgramEvent.silent
-    | read loc _ val _ ord => ProgramEvent.read loc val ord
-    | write loc _ _ val _ ord => ProgramEvent.write loc val ord
-    | update loc _ _ valr valw _ _ ordr ordw => ProgramEvent.update loc valr valw ordr ordw
-    | fence ordr ordw => ProgramEvent.fence ordr ordw
-    | syscall ev => ProgramEvent.syscall ev
-    | failure => ProgramEvent.failure
-    end.
-
-  Definition get_machine_event (e: t): MachineEvent.t :=
-    match e with
-    | syscall e => MachineEvent.syscall e
-    | failure => MachineEvent.failure
-    | _ => MachineEvent.silent
-    end.
-
-  Definition is_promising (e:t) : option (Loc.t * Time.t) :=
-    match e with
-    | promise loc from to msg kind => Some (loc, to)
-    | _ => None
-    end.
-
-  Definition is_reading (e:t): option (Loc.t * Time.t * Const.t * option View.t * Ordering.t) :=
-    match e with
-    | read loc ts val released ord => Some (loc, ts, val, released, ord)
-    | update loc tsr _ valr _ releasedr _ ordr _ => Some (loc, tsr, valr, releasedr, ordr)
-    | _ => None
-    end.
-
-  Definition is_writing (e:t): option (Loc.t * Time.t * Time.t * Const.t * option View.t * Ordering.t) :=
-    match e with
-    | write loc from to val released ord => Some (loc, from, to, val, released, ord)
-    | update loc tsr tsw _ valw _ releasedw _ ordw => Some (loc, tsr, tsw, valw, releasedw, ordw)
-    | _ => None
-    end.
-
-  Definition is_accessing (e:t): option (Loc.t * Time.t) :=
-    match e with
-    | read loc ts _ _ _ => Some (loc, ts)
-    | write loc _ ts _ _ _ => Some (loc, ts)
-    | update loc _ ts _ _ _ _ _ _ => Some (loc, ts)
-    | _ => None
-    end.
-
-  Inductive le: forall (lhs rhs:t), Prop :=
-  | le_promise
-      loc from to msg1 msg2 kind1 kind2
-      (LEREL: Message.le msg1 msg2):
-      le (promise loc from to msg1 kind1) (promise loc from to msg2 kind2)
-  | le_silent:
-      le silent silent
-  | le_read
-      loc ts val rel1 rel2 ord
-      (LEREL: View.opt_le rel1 rel2):
-      le (read loc ts val rel1 ord) (read loc ts val rel2 ord)
-  | le_write
-      loc from to val rel1 rel2 ord
-      (LEREL: View.opt_le rel1 rel2):
-      le (write loc from to val rel1 ord) (write loc from to val rel2 ord)
-  | le_update
-      loc tsr tsw valr valw relr1 relr2 relw1 relw2 ordr ordw
-      (LEREL: View.opt_le relr1 relr2)
-      (LEREL: View.opt_le relw1 relw2):
-      le (update loc tsr tsw valr valw relr1 relw1 ordr ordw) (update loc tsr tsw valr valw relr2 relw2 ordr ordw)
-  | le_fence ordr ordw:
-      le (fence ordr ordw) (fence ordr ordw)
-  | le_syscall e:
-      le (syscall e) (syscall e)
-  | le_failure:
-      le failure failure
-  .
-  Hint Constructors le.
-
-  Definition lift (ord0:Ordering.t) (e:t): t :=
-    match e with
-    | promise loc from to msg kind =>
-      promise loc from to msg kind
-    | silent => silent
-    | read loc ts val released ord =>
-      read loc ts val released (Ordering.join ord0 ord)
-    | write loc from to val released ord =>
-      write loc from to val released (Ordering.join ord0 ord)
-    | update loc tsr tsw valr valw releasedr releasedw ordr ordw =>
-      update loc tsr tsw valr valw releasedr releasedw (Ordering.join ord0 ordr) (Ordering.join ord0 ordw)
-    | fence ordr ordw =>
-      fence (Ordering.join ord0 ordr) (Ordering.join ord0 ordw)
-    | syscall e =>
-      syscall e
-    | failure =>
-      failure
-    end.
-
-  Lemma lift_plain e:
-    lift Ordering.plain e = e.
-  Proof. destruct e; ss. Qed.
-
-End ThreadEvent.
-
-Module Local.
-  Structure t := mk {
-    tview: TView.t;
-    promises: Memory.t;
-  }.
-
-  Definition init := mk TView.bot Memory.bot.
-
-  Inductive is_terminal (lc:t): Prop :=
-  | is_terminal_intro
-      (PROMISES: lc.(promises) = Memory.bot)
-  .
-  Hint Constructors is_terminal.
-
-  Inductive wf (lc:t) (mem:Memory.t): Prop :=
-  | wf_intro
-      (TVIEW_WF: TView.wf lc.(tview))
-      (TVIEW_CLOSED: TView.closed lc.(tview) mem)
-      (PROMISES: Memory.le lc.(promises) mem)
-      (FINITE: Memory.finite lc.(promises))
-      (BOT: Memory.bot_none lc.(promises))
-      (RESERVE: Memory.reserve_wf lc.(promises) mem)
-  .
-  Hint Constructors wf.
-
-  Lemma cap_wf
-        lc promises mem1 mem2
-        (CAP: Memory.cap promises mem1 mem2)
-        (WF: wf lc mem1):
-    wf lc mem2.
-  Proof.
-    inv WF. econs; eauto.
-    - eapply TView.cap_closed; eauto.
-    - eapply Memory.cap_le; eauto.
-    - eapply Memory.cap_reserve_wf; eauto.
-  Qed.
-
-  Inductive disjoint (lc1 lc2:t): Prop :=
-  | disjoint_intro
-      (DISJOINT: Memory.disjoint lc1.(promises) lc2.(promises))
-  .
-  Hint Constructors disjoint.
-
-  Global Program Instance disjoint_Symmetric: Symmetric disjoint.
-  Next Obligation.
-    econs. symmetry. apply H.
-  Qed.
-
-  Definition promise_consistent (lc:t): Prop :=
-    forall loc ts from val released
-       (PROMISE: Memory.get loc ts lc.(promises) = Some (from, Message.full val released)),
-      Time.lt (lc.(tview).(TView.cur).(View.rlx) loc) ts.
-
-  Lemma bot_promise_consistent
-        lc
-        (PROMISES: lc.(promises) = Memory.bot):
-    promise_consistent lc.
-  Proof.
-    ii. rewrite PROMISES, Memory.bot_get in *. ss.
-  Qed.
-
-  Lemma terminal_promise_consistent
-        lc
-        (TERMINAL: is_terminal lc):
-    promise_consistent lc.
-  Proof.
-    inv TERMINAL. apply bot_promise_consistent. auto.
-  Qed.
-
-
-  Inductive promise_step (lc1:t) (mem1:Memory.t) (loc:Loc.t) (from to:Time.t) (msg:Message.t) (lc2:t) (mem2:Memory.t) (kind:Memory.op_kind): Prop :=
+Module ALocal.
+  Inductive promise_step (lc1:Local.t) (mem1:Memory.t) (loc:Loc.t) (from to:Time.t) (msg:Message.t) (lc2:Local.t) (mem2:Memory.t) (kind:Memory.op_kind): Prop :=
   | promise_step_intro
       promises2
-      (PROMISE: Memory.promise lc1.(promises) mem1 loc from to msg promises2 mem2 kind)
+      (PROMISE: AMemory.promise lc1.(Local.promises) mem1 loc from to msg promises2 mem2 kind)
       (CLOSED: Memory.closed_message msg mem2)
-      (LC2: lc2 = mk lc1.(tview) promises2):
+      (LC2: lc2 = Local.mk lc1.(Local.tview) promises2):
       promise_step lc1 mem1 loc from to msg lc2 mem2 kind
   .
   Hint Constructors promise_step.
 
-  Inductive read_step (lc1:t) (mem1:Memory.t) (loc:Loc.t) (to:Time.t) (val:Const.t) (released:option View.t) (ord:Ordering.t) (lc2:t): Prop :=
-  | read_step_intro
-      from
-      tview2
-      (GET: Memory.get loc to mem1 = Some (from, Message.full val released))
-      (READABLE: TView.readable lc1.(tview).(TView.cur) loc to released ord)
-      (TVIEW: TView.read_tview lc1.(tview) loc to released ord = tview2)
-      (LC2: lc2 = mk tview2 lc1.(promises)):
-      read_step lc1 mem1 loc to val released ord lc2
-  .
-  Hint Constructors read_step.
-
-  Inductive write_step (lc1:t) (sc1:TimeMap.t) (mem1:Memory.t) (loc:Loc.t) (from to:Time.t) (val:Const.t) (releasedm released:option View.t) (ord:Ordering.t) (lc2:t) (sc2:TimeMap.t) (mem2:Memory.t) (kind:Memory.op_kind): Prop :=
+  Inductive write_step (lc1:Local.t) (sc1:TimeMap.t) (mem1:Memory.t) (loc:Loc.t) (from to:Time.t) (val:Const.t) (releasedm released:option View.t) (ord:Ordering.t) (lc2:Local.t) (sc2:TimeMap.t) (mem2:Memory.t) (kind:Memory.op_kind): Prop :=
   | write_step_intro
       promises2
-      (RELEASED: released = TView.write_released lc1.(tview) sc1 loc to releasedm ord)
-      (WRITABLE: TView.writable lc1.(tview).(TView.cur) sc1 loc to ord)
-      (WRITE: Memory.write lc1.(promises) mem1 loc from to val released promises2 mem2 kind)
-      (RELEASE: Ordering.le Ordering.strong_relaxed ord -> Memory.nonsynch_loc loc lc1.(promises))
-      (LC2: lc2 = mk (TView.write_tview lc1.(tview) sc1 loc to ord) promises2)
+      (RELEASED: released = TView.write_released lc1.(Local.tview) sc1 loc to releasedm ord)
+      (WRITABLE: TView.writable lc1.(Local.tview).(TView.cur) sc1 loc to ord)
+      (WRITE: AMemory.write lc1.(Local.promises) mem1 loc from to val released promises2 mem2 kind)
+      (RELEASE: Ordering.le Ordering.strong_relaxed ord -> Memory.nonsynch_loc loc lc1.(Local.promises))
+      (LC2: lc2 = Local.mk (TView.write_tview lc1.(Local.tview) sc1 loc to ord) promises2)
       (SC2: sc2 = sc1):
       write_step lc1 sc1 mem1 loc from to val releasedm released ord lc2 sc2 mem2 kind
   .
   Hint Constructors write_step.
-
-  Inductive fence_step (lc1:t) (sc1:TimeMap.t) (ordr ordw:Ordering.t) (lc2:t) (sc2:TimeMap.t): Prop :=
-  | fence_step_intro
-      tview2
-      (READ: TView.read_fence_tview lc1.(tview) ordr = tview2)
-      (RELEASE: Ordering.le Ordering.strong_relaxed ordw -> Memory.nonsynch lc1.(promises))
-      (LC2: lc2 = mk (TView.write_fence_tview tview2 sc1 ordw) lc1.(promises))
-      (SC2: sc2 = TView.write_fence_sc tview2 sc1 ordw):
-      fence_step lc1 sc1 ordr ordw lc2 sc2
-  .
-  Hint Constructors fence_step.
-
-  Inductive failure_step (lc1:t): Prop :=
-  | failure_step_intro
-      (CONSISTENT: promise_consistent lc1)
-  .
-  Hint Constructors failure_step.
 
   Inductive program_step: forall (e:ThreadEvent.t) lc1 sc1 mem1 lc2 sc2 mem2, Prop :=
   | step_silent
@@ -300,7 +63,7 @@ Module Local.
   | step_write
       lc1 sc1 mem1
       loc from to val released ord lc2 sc2 mem2 kind
-      (LOCAL: Local.write_step lc1 sc1 mem1 loc from to val None released ord lc2 sc2 mem2 kind):
+      (LOCAL: write_step lc1 sc1 mem1 loc from to val None released ord lc2 sc2 mem2 kind):
       program_step (ThreadEvent.write loc from to val released ord) lc1 sc1 mem1 lc2 sc2 mem2
   | step_update
       lc1 sc1 mem1
@@ -308,7 +71,7 @@ Module Local.
       tsr valr releasedr releasedw lc2
       tsw valw lc3 sc3 mem3 kind
       (LOCAL1: Local.read_step lc1 mem1 loc tsr valr releasedr ordr lc2)
-      (LOCAL2: Local.write_step lc2 sc1 mem1 loc tsr tsw valw releasedr releasedw ordw lc3 sc3 mem3 kind):
+      (LOCAL2: write_step lc2 sc1 mem1 loc tsr tsw valw releasedr releasedw ordw lc3 sc3 mem3 kind):
       program_step (ThreadEvent.update loc tsr tsw valr valw releasedr releasedw ordr ordw) lc1 sc1 mem1 lc3 sc3 mem3
   | step_fence
       lc1 sc1 mem1
@@ -333,20 +96,20 @@ Module Local.
   Lemma promise_step_future
         lc1 sc1 mem1 loc from to msg lc2 mem2 kind
         (STEP: promise_step lc1 mem1 loc from to msg lc2 mem2 kind)
-        (WF1: wf lc1 mem1)
+        (WF1: Local.wf lc1 mem1)
         (SC1: Memory.closed_timemap sc1 mem1)
         (CLOSED1: Memory.closed mem1):
-    <<WF2: wf lc2 mem2>> /\
+    <<WF2: Local.wf lc2 mem2>> /\
     <<SC2: Memory.closed_timemap sc1 mem2>> /\
     <<CLOSED2: Memory.closed mem2>> /\
     <<FUTURE: Memory.future mem1 mem2>> /\
-    <<TVIEW_FUTURE: TView.le lc1.(tview) lc2.(tview)>> /\
+    <<TVIEW_FUTURE: TView.le lc1.(Local.tview) lc2.(Local.tview)>> /\
     <<MSG_WF: Message.wf msg>> /\
     <<MSG_TS: Memory.message_to msg loc to>> /\
     <<MSG_CLOSED: Memory.closed_message msg mem2>>.
   Proof.
     inv WF1. inv STEP.
-    exploit Memory.promise_future; eauto. i. des.
+    exploit AMemory.promise_future; eauto. i. des.
     splits; ss.
     - econs; ss. eapply TView.future_closed; eauto.
     - eapply Memory.future_closed_timemap; eauto.
@@ -359,37 +122,18 @@ Module Local.
     - by inv PROMISE.
   Qed.
 
-  Lemma read_step_future
-        lc1 mem1 loc ts val released ord lc2
-        (STEP: read_step lc1 mem1 loc ts val released ord lc2)
-        (WF1: wf lc1 mem1)
-        (CLOSED1: Memory.closed mem1):
-    <<WF2: wf lc2 mem1>> /\
-    <<TVIEW_FUTURE: TView.le lc1.(tview) lc2.(tview)>> /\
-    <<REL_WF: View.opt_wf released>> /\
-    <<REL_CLOSED: Memory.closed_opt_view released mem1>>.
-  Proof.
-    inv WF1. inv STEP.
-    dup CLOSED1. inv CLOSED0. exploit CLOSED; eauto. i. des.
-    inv MSG_WF. inv MSG_CLOSED.
-    exploit TViewFacts.read_future; try exact GET; eauto.
-    i. des. splits; auto.
-    - econs; eauto.
-    - apply TViewFacts.read_tview_incr.
-  Qed.
-
   Lemma write_step_future
         lc1 sc1 mem1 loc from to val releasedm released ord lc2 sc2 mem2 kind
         (STEP: write_step lc1 sc1 mem1 loc from to val releasedm released ord lc2 sc2 mem2 kind)
         (REL_WF: View.opt_wf releasedm)
         (REL_CLOSED: Memory.closed_opt_view releasedm mem1)
-        (WF1: wf lc1 mem1)
+        (WF1: Local.wf lc1 mem1)
         (SC1: Memory.closed_timemap sc1 mem1)
         (CLOSED1: Memory.closed mem1):
-    <<WF2: wf lc2 mem2>> /\
+    <<WF2: Local.wf lc2 mem2>> /\
     <<SC2: Memory.closed_timemap sc2 mem2>> /\
     <<CLOSED2: Memory.closed mem2>> /\
-    <<TVIEW_FUTURE: TView.le lc1.(tview) lc2.(tview)>> /\
+    <<TVIEW_FUTURE: TView.le lc1.(Local.tview) lc2.(Local.tview)>> /\
     <<SC_FUTURE: TimeMap.le sc1 sc2>> /\
     <<MEM_FUTURE: Memory.future mem1 mem2>> /\
     <<REL_WF: View.opt_wf released>> /\
@@ -398,10 +142,10 @@ Module Local.
   Proof.
     inv WF1. inv STEP.
     exploit TViewFacts.write_future; eauto.
-    { inv WRITE. eapply Memory.promise_op. eauto. }
+    { inv WRITE. eapply AMemory.promise_op. eauto. }
     s. i. des.
-    exploit Memory.write_future; try apply WRITE; eauto. i. des.
-    exploit Memory.write_get2; try apply WRITE; eauto; try by viewtac. i. des.
+    exploit AMemory.write_future; try apply WRITE; eauto. i. des.
+    exploit AMemory.write_get2; try apply WRITE; eauto; try by viewtac. i. des.
     splits; eauto.
     - apply TViewFacts.write_tview_incr. auto.
     - refl.
@@ -423,52 +167,30 @@ Module Local.
     revert H0. unfold TView.write_released. condtac; ss. by destruct ord.
   Qed.
 
-  Lemma fence_step_future
-        lc1 sc1 mem1 ordr ordw lc2 sc2
-        (STEP: fence_step lc1 sc1 ordr ordw lc2 sc2)
-        (WF1: wf lc1 mem1)
-        (SC1: Memory.closed_timemap sc1 mem1)
-        (CLOSED1: Memory.closed mem1):
-    <<WF2: wf lc2 mem1>> /\
-    <<SC2: Memory.closed_timemap sc2 mem1>> /\
-    <<TVIEW_FUTURE: TView.le lc1.(tview) lc2.(tview)>> /\
-    <<SC_FUTURE: TimeMap.le sc1 sc2>>.
-  Proof.
-    inv WF1. inv STEP.
-    exploit TViewFacts.read_fence_future; eauto. i. des.
-    exploit TViewFacts.write_fence_future; eauto. i. des.
-    splits; eauto.
-    - etrans.
-      + apply TViewFacts.write_fence_tview_incr. auto.
-      + apply TViewFacts.write_fence_tview_mon; eauto; try refl.
-        apply TViewFacts.read_fence_tview_incr. auto.
-    - apply TViewFacts.write_fence_sc_incr.
-  Qed.
-
   Lemma program_step_future
         e lc1 sc1 mem1 lc2 sc2 mem2
         (STEP: program_step e lc1 sc1 mem1 lc2 sc2 mem2)
-        (WF1: wf lc1 mem1)
+        (WF1: Local.wf lc1 mem1)
         (SC1: Memory.closed_timemap sc1 mem1)
         (CLOSED1: Memory.closed mem1):
-    <<WF2: wf lc2 mem2>> /\
+    <<WF2: Local.wf lc2 mem2>> /\
     <<SC2: Memory.closed_timemap sc2 mem2>> /\
     <<CLOSED2: Memory.closed mem2>> /\
-    <<TVIEW_FUTURE: TView.le lc1.(tview) lc2.(tview)>> /\
+    <<TVIEW_FUTURE: TView.le lc1.(Local.tview) lc2.(Local.tview)>> /\
     <<SC_FUTURE: TimeMap.le sc1 sc2>> /\
     <<MEM_FUTURE: Memory.future mem1 mem2>>.
   Proof.
     inv STEP.
     - esplits; eauto; try refl.
-    - exploit read_step_future; eauto. i. des.
+    - exploit Local.read_step_future; eauto. i. des.
       esplits; eauto; try refl.
     - exploit write_step_future; eauto; try by econs. i. des.
       esplits; eauto; try refl.
-    - exploit read_step_future; eauto. i. des.
+    - exploit Local.read_step_future; eauto. i. des.
       exploit write_step_future; eauto; try by econs. i. des.
       esplits; eauto. etrans; eauto.
-    - exploit fence_step_future; eauto. i. des. esplits; eauto; try refl.
-    - exploit fence_step_future; eauto. i. des. esplits; eauto; try refl.
+    - exploit Local.fence_step_future; eauto. i. des. esplits; eauto; try refl.
+    - exploit Local.fence_step_future; eauto. i. des. esplits; eauto; try refl.
     - esplits; eauto; try refl.
   Qed.
 
@@ -501,90 +223,58 @@ Module Local.
   Lemma promise_step_disjoint
         lc1 sc1 mem1 loc from to msg lc2 mem2 lc kind
         (STEP: promise_step lc1 mem1 loc from to msg lc2 mem2 kind)
-        (WF1: wf lc1 mem1)
+        (WF1: Local.wf lc1 mem1)
         (SC1: Memory.closed_timemap sc1 mem1)
         (CLOSED1: Memory.closed mem1)
-        (DISJOINT1: disjoint lc1 lc)
-        (WF: wf lc mem1):
-    <<DISJOINT2: disjoint lc2 lc>> /\
-    <<WF: wf lc mem2>>.
+        (DISJOINT1: Local.disjoint lc1 lc)
+        (WF: Local.wf lc mem1):
+    <<DISJOINT2: Local.disjoint lc2 lc>> /\
+    <<WF: Local.wf lc mem2>>.
   Proof.
     inv WF1. inv DISJOINT1. inversion WF. inv STEP.
-    exploit Memory.promise_future; try apply PROMISE; eauto. i. des.
-    exploit Memory.promise_disjoint; try apply PROMISE; eauto. i. des.
+    exploit AMemory.promise_future; try apply PROMISE; eauto. i. des.
+    exploit AMemory.promise_disjoint; try apply PROMISE; eauto. i. des.
     splits; ss. econs; eauto.
     eapply TView.future_closed; eauto.
-  Qed.
-
-  Lemma read_step_disjoint
-        lc1 mem1 lc2 loc ts val released ord lc
-        (STEP: read_step lc1 mem1 loc ts val released ord lc2)
-        (WF1: wf lc1 mem1)
-        (DISJOINT1: disjoint lc1 lc)
-        (WF: wf lc mem1):
-    disjoint lc2 lc.
-  Proof.
-    inv WF1. inv DISJOINT1. inv WF. inv STEP. ss.
   Qed.
 
   Lemma write_step_disjoint
         lc1 sc1 mem1 lc2 sc2 loc from to val releasedm released ord mem2 kind lc
         (STEP: write_step lc1 sc1 mem1 loc from to val releasedm released ord lc2 sc2 mem2 kind)
-        (WF1: wf lc1 mem1)
+        (WF1: Local.wf lc1 mem1)
         (SC1: Memory.closed_timemap sc1 mem1)
         (CLOSED1: Memory.closed mem1)
-        (DISJOINT1: disjoint lc1 lc)
-        (WF: wf lc mem1):
-    <<DISJOINT2: disjoint lc2 lc>> /\
-    <<WF: wf lc mem2>>.
+        (DISJOINT1: Local.disjoint lc1 lc)
+        (WF: Local.wf lc mem1):
+    <<DISJOINT2: Local.disjoint lc2 lc>> /\
+    <<WF: Local.wf lc mem2>>.
   Proof.
     inv WF1. inv DISJOINT1. inversion WF. inv STEP.
-    exploit Memory.write_disjoint; try apply WRITE; eauto. i. des.
+    exploit AMemory.write_disjoint; try apply WRITE; eauto. i. des.
     splits; ss. econs; eauto.
-    inv WRITE. eapply TView.promise_closed; eauto.
-  Qed.
-
-  Lemma fence_step_disjoint
-        lc1 sc1 mem1 lc2 sc2 ordr ordw lc
-        (STEP: fence_step lc1 sc1 ordr ordw lc2 sc2)
-        (WF1: wf lc1 mem1)
-        (SC1: Memory.closed_timemap sc1 mem1)
-        (DISJOINT1: disjoint lc1 lc)
-        (WF: wf lc mem1):
-    <<DISJOINT2: disjoint lc2 lc>> /\
-    <<WF: wf lc mem1>>.
-  Proof.
-    inv WF1. inv DISJOINT1. inv WF. inv STEP. splits; ss.
-  Qed.
-
-  Lemma read_step_promises
-        lc1 mem loc to val released ord lc2
-        (READ: read_step lc1 mem loc to val released ord lc2):
-    lc1.(promises) = lc2.(promises).
-  Proof.
-    inv READ. auto.
+    inv WRITE. eapply ATView.promise_closed; eauto.
   Qed.
 
   Lemma program_step_disjoint
         e lc1 sc1 mem1 lc2 sc2 mem2 lc
         (STEP: program_step e lc1 sc1 mem1 lc2 sc2 mem2)
-        (WF1: wf lc1 mem1)
+        (WF1: Local.wf lc1 mem1)
         (SC1: Memory.closed_timemap sc1 mem1)
         (CLOSED1: Memory.closed mem1)
-        (DISJOINT1: disjoint lc1 lc)
-        (WF: wf lc mem1):
-    <<DISJOINT2: disjoint lc2 lc>> /\
-    <<WF: wf lc mem2>>.
+        (DISJOINT1: Local.disjoint lc1 lc)
+        (WF: Local.wf lc mem1):
+    <<DISJOINT2: Local.disjoint lc2 lc>> /\
+    <<WF: Local.wf lc mem2>>.
   Proof.
     inv STEP.
     - esplits; eauto.
-    - exploit read_step_disjoint; eauto.
+    - exploit Local.read_step_disjoint; eauto.
     - exploit write_step_disjoint; eauto.
-    - exploit read_step_future; eauto. i. des.
-      exploit read_step_disjoint; eauto. i. des.
+    - exploit Local.read_step_future; eauto. i. des.
+      exploit Local.read_step_disjoint; eauto. i. des.
       exploit write_step_disjoint; eauto.
-    - exploit fence_step_disjoint; eauto.
-    - exploit fence_step_disjoint; eauto.
+    - exploit Local.fence_step_disjoint; eauto.
+    - exploit Local.fence_step_disjoint; eauto.
     - esplits; eauto.
   Qed.
 
@@ -594,48 +284,48 @@ Module Local.
   Lemma promise_step_no_reserve_except
         lc1 mem1 loc from to msg lc2 mem2 kind
         (STEP: promise_step lc1 mem1 loc from to msg lc2 mem2 kind)
-        (RESERVE1: Memory.reserve_wf lc1.(promises) mem1)
-        (NORESERVE1: Memory.no_reserve_except lc1.(promises) mem1):
-    Memory.no_reserve_except lc2.(promises) mem2.
+        (RESERVE1: Memory.reserve_wf lc1.(Local.promises) mem1)
+        (NORESERVE1: Memory.no_reserve_except lc1.(Local.promises) mem1):
+    Memory.no_reserve_except lc2.(Local.promises) mem2.
   Proof.
     ii. inv STEP. s.
-    eapply Memory.promise_no_reserve_except; eauto.
+    eapply AMemory.promise_no_reserve_except; eauto.
   Qed.
 
   Lemma program_step_no_reserve_except
         e lc1 sc1 mem1 lc2 sc2 mem2
         (STEP: program_step e lc1 sc1 mem1 lc2 sc2 mem2)
-        (RESERVE1: Memory.reserve_wf lc1.(promises) mem1)
-        (NORESERVE1: Memory.no_reserve_except lc1.(promises) mem1):
-    Memory.no_reserve_except lc2.(promises) mem2.
+        (RESERVE1: Memory.reserve_wf lc1.(Local.promises) mem1)
+        (NORESERVE1: Memory.no_reserve_except lc1.(Local.promises) mem1):
+    Memory.no_reserve_except lc2.(Local.promises) mem2.
   Proof.
     ii. inv STEP; try inv LOCAL; eauto; ss.
     - inv WRITE.
       erewrite Memory.remove_o; eauto. condtac; ss.
       + des. subst.
-        exploit Memory.promise_get0; eauto.
+        exploit AMemory.promise_get0; eauto.
         { inv PROMISE; ss. }
         i. des. congr.
-      + eapply Memory.promise_no_reserve_except; eauto.
+      + eapply AMemory.promise_no_reserve_except; eauto.
     - inv LOCAL1. inv LOCAL2. inv WRITE. ss.
       erewrite Memory.remove_o; eauto. condtac; ss.
       + des. subst.
-        exploit Memory.promise_get0; eauto.
+        exploit AMemory.promise_get0; eauto.
         { inv PROMISE; ss. }
         i. des. congr.
-      + eapply Memory.promise_no_reserve_except; eauto.
+      + eapply AMemory.promise_no_reserve_except; eauto.
   Qed.
 
 
   Lemma bot_program_step_bot
         e lc1 sc1 mem1 lc2 sc2 mem2
         (STEP: program_step e lc1 sc1 mem1 lc2 sc2 mem2)
-        (PROMISES: lc1.(promises) = Memory.bot):
-    lc2.(promises) = Memory.bot.
+        (PROMISES: lc1.(Local.promises) = Memory.bot):
+    lc2.(Local.promises) = Memory.bot.
   Proof.
     inv STEP; try inv LOCAL; ss.
-    - eapply Memory.bot_write_bot; eauto.
+    - eapply AMemory.bot_write_bot; eauto.
     - inv LOCAL1. inv LOCAL2.
-      eapply Memory.bot_write_bot; eauto.
+      eapply AMemory.bot_write_bot; eauto.
   Qed.
-End Local.
+End ALocal.
